

Isomorphism is an Equivalence Relation

Proof Walkthrough

Adam Grant

November 17, 2021

Isomorphic

The nicest definition of isomorphism I've seen is by Roland Backhouse:

Definition

Object x and y in the same category are said to be *isomorphic* if there are two arrows $f \in x \leftarrow y$ and $g \in y \leftarrow x$ such that $f \cdot g = id_x$ and $g \cdot f = id_y$, i.e. they are each other's inverses. If this is the case we write $x \cong y$ or, if we want to be explicit about the arrows, we write $f \in x \cong y \ni g$.

In this presentation, we will be explicit about the arrows. We'll also make the existential quantification explicit and write:

$$x \cong y \equiv \exists(f, g :: f \in x \cong y \ni g)$$

which will help when writing proofs.

Our task

Show that \cong is an *equivalence relation*.

Equivalence Relation

Definition (equivalence relation)

A relation is an *equivalence relation* if it is *reflexive*, *symmetric*, and *transitive*.

Equivalence Relation

Definition (reflexive)

A relation R is *reflexive* when $\forall(a :: aRa)$.

Definition (symmetric)

A relation R is *symmetric* when $\forall(b, a : bRa : aRb)$.

Definition (transitive)

A relation R is *transitive* when $\forall(c, b, a : cRb \wedge bRa : cRa)$.

Proof obligations

Show that \cong is an Equivalence Relation

- Reflexivity: $\forall(a :: a \cong a)$
- Symmetry: $\forall(b, a : b \cong a : a \cong b)$
- Transitivity: $\forall(c, b, a : c \cong b \wedge b \cong a : c \cong a)$

Reflexivity: $\forall(a :: a \cong a)$

- $a \cong a$

\equiv Definition of \cong

$$\exists(f, g :: f \in a \cong a \ni g)$$

\equiv Expand abbreviation

$$\exists(f, g :: f \cdot g = id_a \wedge g \cdot f = id_a)$$

\Leftarrow \exists -introduction, with $f, g := id_a, id_a$

$$id_a \cdot id_a = id_a \wedge id_a \cdot id_a = id_a$$

\equiv \wedge -idempotent

$$id_a \cdot id_a = id_a$$



Proof obligations

Show that \cong is an Equivalence Relation

- ✓ Reflexivity: $\forall(a :: a \cong a)$
- Symmetry: $\forall(b, a : b \cong a : a \cong b)$
- Transitivity: $\forall(c, b, a : c \cong b \wedge b \cong a : c \cong a)$

Symmetry: $\forall(b, a : b \cong a : a \cong b)$

- $b \cong a$

≡ Definition of \cong

$$\exists(f, g :: f \in b \cong a \ni g)$$

≡ Expand abbreviation

$$\exists(f, g :: f \cdot g = id_b \wedge g \cdot f = id_a)$$

≡ \wedge -symmetric; Rearrange dummies

$$\exists(g, f :: g \cdot f = id_a \wedge f \cdot g = id_b)$$

≡ Abbreviate

$$\exists(g, f :: g \in a \cong b \ni f)$$

≡ Definition of \cong

$$a \cong b$$



Proof obligations

Show that \cong is an Equivalence Relation

- ✓ Reflexivity: $\forall(a :: a \cong a)$
- ✓ Symmetry: $\forall(b, a : b \cong a : a \cong b)$
- Transitivity: $\forall(c, b, a : c \cong b \wedge b \cong a : c \cong a)$

Transitivity: $\forall(c, b, a : c \cong b \wedge b \cong a : c \cong a)$

- $b \cong a$

Context

- $c \cong b$
- $b \cong a$

Building Context

Context

- $c \cong b$
- $b \cong a$
- + $\exists(f, g :: f \in c \cong b \ni g)$
- + $\exists(f, g :: f \in b \cong a \ni g)$
- + Define f, g
 $f \in c \cong b \ni g$
 $f \cdot g = id_c \wedge g \cdot f = id_b$
- + Define h, j
 $h \in b \cong a \ni j$
 $h \cdot j = id_b \wedge j \cdot h = id_a$

Building Context

Express id_c in terms of f, g, h, k

- id_c
- = Definition of f, g
 $f \cdot g$
- = Identity
 $f \cdot id_b \cdot g$
- = Definition of h, j
 $f \cdot h \cdot j \cdot g$



Building Context

Context

...

+ Define f, g

$$f \in c \cong b \ni g$$

$$f \cdot g = id_c \wedge g \cdot f = id_b$$

+ Define h, j

$$h \in b \cong a \ni j$$

$$h \cdot j = id_b \wedge j \cdot h = id_a$$

+ $id_c = f.h.j.k$

Building Context

Express id_a in terms of f, g, h, k

- id_a
 - = Definition of h, j
 $j \cdot h$
 - = Identity
 $j \cdot id_b \cdot h$
 - = Definition of h, j
 $j \cdot g \cdot f \cdot h$
-

Building Context

Context

...

$$+ id_c = f \cdot h \cdot j \cdot g$$

$$+ id_a = j \cdot g \cdot f \cdot h$$

Transitivity: $\forall(c, b, a : c \cong b \wedge b \cong a : c \cong a)$

- $b \cong a$

≡ Definition of \cong

$$\exists(f, g :: f \in c \cong a \ni g)$$

≡ Expand abbreviation

$$\exists(f, g :: f \cdot g = id_c \wedge g \cdot f = id_a)$$

← \exists -introduction

$$(f \cdot g = id_c \wedge g \cdot f = id_a)[f, g := f \cdot h, j \cdot g]$$

≡ Textual substitution

$$(f \cdot h) \cdot (j \cdot g) = id_c \wedge (j \cdot g) \cdot (f \cdot h) = id_a$$

≡ Context

true



Proof obligations

Show that \cong is an Equivalence Relation

- ✓ Reflexivity: $\forall(a :: a \cong a)$
- ✓ Symmetry: $\forall(b, a : b \cong a : a \cong b)$
- ✓ Transitivity: $\forall(c, b, a : c \cong b \wedge b \cong a : c \cong a)$